examples/l3-machine-code/m0/prog/m0_progLib.sig
@@ -1,6 +1,7 @@
 signature m0_progLib =
 sig
    val addInstructionClass: string -> bool
+   val get_code: Thm.thm -> Term.term
 
    val m0_config: bool * bool -> unit
    val m0_spec: string -> Thm.thm list
