examples/l3-machine-code/m0/prog/m0_progScript.sml
@@ -1,12 +1,16 @@
 open HolKernel boolLib bossLib
-open stateLib m0_stepTheory
+open lcsymtacs blastLib stateLib set_sepTheory progTheory m0_stepTheory
 
 val () = new_theory "m0_prog"
 
+infix \\
+val op \\ = op THEN;
+
 (* ------------------------------------------------------------------------ *)
 
-val _ = stateLib.sep_definitions "m0" [["PSR"], ["CONTROL"]] [["pcinc"]]
-           m0_stepTheory.NextStateM0_def
+val _ = stateLib.sep_definitions "m0"
+          [["PSR"], ["CONTROL"], ["AIRCR"]] [["pcinc"]]
+          m0_stepTheory.NextStateM0_def
 
 val m0_instr_def = Define`
   (m0_instr (a, INL (opc16: word16)) =
@@ -26,6 +30,65 @@ val M0_IMP_SPEC = Theory.save_thm ("M0_IMP_SPEC",
    stateTheory.IMP_SPEC
    |> Q.ISPECL [`m0_proj`, `NextStateM0`, `m0_instr`]
    |> REWRITE_RULE [GSYM M0_MODEL_def]
+   )
+
+(* ------------------------------------------------------------------------ *)
+
+val m0_REG_def = DB.definition "m0_REG_def"
+val m0_MEM_def = DB.definition "m0_MEM_def"
+
+val (m0_REGISTERS_def, m0_REGISTERS_INSERT) =
+   stateLib.define_map_component ("m0_REGISTERS", "reg", m0_REG_def)
+
+val (m0_MEMORY_def, m0_MEMORY_INSERT) =
+   stateLib.define_map_component ("m0_MEMORY", "mem", m0_MEM_def)
+
+val m0_CONFIG_def = Define`
+   m0_CONFIG (bigend, spsel) =
+      m0_exception NoException * m0_AIRCR_ENDIANNESS bigend *
+      m0_CONTROL_SPSEL spsel`
+
+val m0_PC_def = Define`
+   m0_PC pc = m0_REG RName_PC pc * cond (Aligned (pc,2))`
+
+val m0_NZCV_def = Define`
+   m0_NZCV (n,z,c,v) = m0_PSR_N n * m0_PSR_Z z * m0_PSR_C c * m0_PSR_V v`
+
+(* ------------------------------------------------------------------------ *)
+
+val m0_NZCV_HIDE = Q.store_thm("m0_NZCV_HIDE",
+   `~m0_NZCV = ~m0_PSR_N * ~m0_PSR_Z * ~m0_PSR_C * ~m0_PSR_V`,
+   SIMP_TAC std_ss [SEP_HIDE_def, m0_NZCV_def, SEP_CLAUSES, FUN_EQ_THM]
+   \\ SIMP_TAC std_ss [SEP_EXISTS]
+   \\ METIS_TAC [m0_NZCV_def, pairTheory.PAIR]
+   )
+
+val m0_PSR_T_F = Q.store_thm("m0_PSR_T_F",
+   `( n ==> (m0_PSR_N T = m0_PSR_N n)) /\
+    (~n ==> (m0_PSR_N F = m0_PSR_N n)) /\
+    ( z ==> (m0_PSR_Z T = m0_PSR_Z z)) /\
+    (~z ==> (m0_PSR_Z F = m0_PSR_Z z)) /\
+    ( c ==> (m0_PSR_C T = m0_PSR_C c)) /\
+    (~c ==> (m0_PSR_C F = m0_PSR_C c)) /\
+    ( v ==> (m0_PSR_V T = m0_PSR_V v)) /\
+    (~v ==> (m0_PSR_V F = m0_PSR_V v))`,
+    simp []
+    )
+
+val m0_PC_INTRO = Q.store_thm("m0_PC_INTRO",
+   `SPEC m (p1 * m0_PC pc) code (p2 * m0_REG RName_PC pc') ==>
+    (Aligned (pc,2) ==> Aligned (pc',2)) ==>
+    SPEC m (p1 * m0_PC pc) code (p2 * m0_PC pc')`,
+   REPEAT STRIP_TAC
+   \\ FULL_SIMP_TAC std_ss [m0_PC_def, SPEC_MOVE_COND, STAR_ASSOC, SEP_CLAUSES]
+   )
+
+val tm = Term.subst [``b0:bool`` |-> boolSyntax.F] (bitstringSyntax.mk_vec 32 0)
+
+val Aligned_Branch = Q.store_thm("Aligned_Branch",
+   `(Aligned (pc:word32, 2) ==> Aligned (pc + 4w + ^tm, 2)) = T`,
+   rw [Aligned]
+   \\ blastLib.FULL_BBLAST_TAC
    )
 
 (* ------------------------------------------------------------------------ *)
